rocq-brick-libstdcpp/proof/cstring/pred.v
@@ -4,6 +4,9 @@
  * See the LICENSE-BedRock file in the repository root for details.
  *)
 Require Import skylabs.auto.cpp.prelude.proof.
+Require Import skylabs.auto.cpp.proof.
+Require Import skylabs.auto.cpp.hints.anyR.
+Require Import skylabs.cpp.array.
 Require Export skylabs.cpp.string.
 Require Export skylabs.brick.libstdcpp.cstring.model.
 
@@ -49,3 +52,527 @@ Axiom object_bytes_anyR_of_anyR_array : forall `{Σ : cpp_logic} {σ : genv}
     (p : ptr) ty n,
   p |-> anyR (Tarray ty n) 1$m ⊢
   p |-> object_bytes_anyR ty (Z.of_N n).
+
+Lemma borrow_arrayR_cstringR `{Σ : cpp_logic, σ : genv}
+    (p : ptr) q bytes s tail :
+  bytes = cstring.to_zstring s ++ tail ->
+  cstring.WF s ->
+  p |-> arrayR (Tchar_ char_type.Cchar) (fun c : N => charR q c)
+          bytes ⊢
+  p |-> cstring.R q s ∗
+  (p |-> cstring.R q s -∗
+   p |-> arrayR (Tchar_ char_type.Cchar) (fun c : N => charR q c)
+           bytes).
+Proof.
+  intros Hbytes Hwf.
+  subst bytes.
+  rewrite (arrayR_app (fun c : N => charR q c) (Tchar_ char_type.Cchar)).
+  iIntros "[Hs Htail]".
+  iSplitL "Hs".
+  - rewrite /cstring.R /zstring.R. iFrame. done.
+  - iIntros "Hs".
+    rewrite /cstring.R /zstring.R.
+    iDestruct "Hs" as "[Hs _]".
+    iFrame.
+Qed.
+
+Lemma borrow_arrayLR_cstringR `{Σ : cpp_logic, σ : genv}
+    (p : ptr) q bytes s tail :
+  bytes = cstring.to_zstring s ++ tail ->
+  cstring.WF s ->
+  p |-> arrayLR (Tchar_ char_type.Cchar) 0 (lengthZ bytes)
+          (fun c : N => charR q c) bytes ⊢
+  p |-> cstring.R q s ∗
+  (p |-> cstring.R q s -∗
+   p |-> arrayLR (Tchar_ char_type.Cchar) 0 (lengthZ bytes)
+           (fun c : N => charR q c) bytes).
+Proof.
+  intros Hbytes Hwf.
+  rewrite arrayLR.unlock _at_sep.
+  iIntros "[_ Harr]".
+  rewrite _at_offsetR _at_sub_0; [|done].
+  iPoseProof (borrow_arrayR_cstringR p q bytes s tail Hbytes Hwf with "Harr")
+    as "[Hs Hclose]".
+  iSplitL "Hs".
+  - iExact "Hs".
+  - iIntros "Hs".
+    iPoseProof ("Hclose" with "Hs") as "Harr".
+    rewrite /arrayLR.
+    iSplit.
+    + iPureIntro. lia.
+    + iExact "Harr".
+Qed.
+
+Lemma offset_entails `{Σ : cpp_logic, σ : genv}
+    (o : offset) (P Q : Rep) :
+  (P ⊢ Q) -> o |-> P ⊢ o |-> Q.
+Proof.
+  intros HPQ. apply _offsetR_mono. exact HPQ.
+Qed.
+
+Lemma at_zero_intro `{Σ : cpp_logic, σ : genv}
+    (p : ptr) (R : Rep) :
+  p |-> R ⊢ p .[Tuchar ! 0] |-> R.
+Proof.
+  rewrite _at_sub_0; [reflexivity|done].
+Qed.
+
+Lemma at_zero_elim `{Σ : cpp_logic, σ : genv}
+    (p : ptr) (R : Rep) :
+  p .[Tuchar ! 0] |-> R ⊢ p |-> R.
+Proof.
+  rewrite _at_sub_0; [reflexivity|done].
+Qed.
+
+Lemma at_type_ptrR_validR_plus_one `{Σ : cpp_logic, σ : genv}
+    (p : ptr) ty :
+  p |-> type_ptrR ty ⊢ p .[ty ! 1] |-> validR.
+Proof.
+  rewrite -_at_offsetR.
+  apply heap_pred._at_cancel.
+  apply type_ptrR_validR_plus_one.
+Qed.
+
+Lemma at_uchar_offset_add_intro `{Σ : cpp_logic, σ : genv}
+    (p : ptr) i j k (R : Rep) :
+  k = (i + j)%Z ->
+  p .[Tuchar ! k] |-> R ⊢ p .[Tuchar ! i] .[Tuchar ! j] |-> R.
+Proof.
+  intros ->.
+  rewrite o_sub_sub.
+  reflexivity.
+Qed.
+
+Lemma at_uchar_offset_add_elim `{Σ : cpp_logic, σ : genv}
+    (p : ptr) i j k (R : Rep) :
+  k = (i + j)%Z ->
+  p .[Tuchar ! i] .[Tuchar ! j] |-> R ⊢ p .[Tuchar ! k] |-> R.
+Proof.
+  intros ->.
+  rewrite o_sub_sub.
+  reflexivity.
+Qed.
+
+Lemma arrayR_charR_Vchar `{Σ : cpp_logic, σ : genv} q xs :
+  arrayR (Tchar_ char_type.Cchar) (fun c : N => charR q c) xs ⊢
+  arrayR (Tchar_ char_type.Cchar)
+    (fun c : N => primR (Tchar_ char_type.Cchar) q (Vchar c)) xs.
+Proof.
+  induction xs as [| x xs IH].
+  - rewrite !arrayR_nil. iIntros "[$ $]".
+  - rewrite !arrayR_cons.
+    iIntros "[$ [$ Hxs]]".
+    iApply (offset_entails with "Hxs").
+    exact IH.
+Qed.
+
+Lemma at_arrayR_charR_Vchar `{Σ : cpp_logic, σ : genv}
+    (p : ptr) q xs :
+  p |-> arrayR (Tchar_ char_type.Cchar) (fun c : N => charR q c) xs ⊢
+  p |-> arrayR (Tchar_ char_type.Cchar)
+          (fun c : N => primR (Tchar_ char_type.Cchar) q (Vchar c)) xs.
+Proof.
+  apply heap_pred._at_cancel.
+  by apply arrayR_charR_Vchar.
+Qed.
+
+Lemma arrayR_charR_anyR `{Σ : cpp_logic, σ : genv} (p : ptr) n xs :
+  N.to_nat n = length xs ->
+  p |-> arrayR (Tchar_ char_type.Cchar) (fun c : N => charR 1$m c) xs ⊢
+  p |-> anyR (Tarray (Tchar_ char_type.Cchar) n) 1$m.
+Proof.
+  intros Hlen.
+  iIntros "Harr".
+  iPoseProof (at_arrayR_charR_Vchar with "Harr") as "Harr".
+  rewrite anyR_array.
+  iApply (arrayR_anyR_f (fun c : N => Vchar c) with "Harr").
+  exact Hlen.
+Qed.
+
+Lemma arrayLR_charR_anyR `{Σ : cpp_logic, σ : genv} (p : ptr) n xs :
+  N.to_nat n = length xs ->
+  p |-> arrayLR (Tchar_ char_type.Cchar) 0 (Z.of_N n)
+         (fun c : N => charR 1$m c) xs ⊢
+  p |-> anyR (Tarray (Tchar_ char_type.Cchar) n) 1$m.
+Proof.
+  intros Hlen.
+  rewrite arrayLR.unlock _at_sep.
+  iIntros "[_ Harr]".
+  rewrite _at_offsetR _at_sub_0; [|done].
+  iApply (arrayR_charR_anyR with "Harr").
+  exact Hlen.
+Qed.
+
+Lemma at_charR_anyR `{Σ : cpp_logic, σ : genv}
+    (p : ptr) q x :
+  p |-> charR q x ⊢ p |-> anyR (Tchar_ char_type.Cchar) q.
+Proof.
+  apply heap_pred._at_cancel.
+  apply primR_anyR.
+Qed.
+
+Lemma arrayR_charR_arrayR_anyR `{Σ : cpp_logic, σ : genv}
+    (p : ptr) xs :
+  p |-> arrayR (Tchar_ char_type.Cchar) (fun c : N => charR 1$m c) xs ⊢
+  p |-> arrayR (Tchar_ char_type.Cchar)
+         (fun _ : unit => anyR (Tchar_ char_type.Cchar) 1$m)
+         (replicateN (lengthN xs) ()).
+Proof.
+  revert p.
+  induction xs as [|x xs IH].
+  all: intros p.
+  - rewrite /lengthN /= !arrayR_nil. reflexivity.
+  - rewrite arrayR_cons !_at_sep _at_offsetR.
+    iIntros "(Hty & Hx & Hxs)".
+    replace (lengthN (x :: xs)) with (N.succ (lengthN xs)) by
+      (rewrite /lengthN Nat2N.inj_succ; reflexivity).
+    rewrite replicateN_S.
+    rewrite arrayR_cons !_at_sep _at_offsetR.
+    iFrame "Hty".
+    iSplitL "Hx".
+    + iApply (at_charR_anyR with "Hx").
+    + iApply (IH with "Hxs").
+Qed.
+
+Lemma arrayLR_charR_arrayLR_anyR `{Σ : cpp_logic, σ : genv}
+    (p : ptr) n xs :
+  N.to_nat n = length xs ->
+  p |-> arrayLR (Tchar_ char_type.Cchar) 0 (Z.of_N n)
+         (fun c : N => charR 1$m c) xs ⊢
+  p |-> arrayLR (Tchar_ char_type.Cchar) 0 (Z.of_N n)
+         (fun _ : unit => anyR (Tchar_ char_type.Cchar) 1$m)
+         (replicateN n ()).
+Proof.
+  intros Hlen.
+  rewrite arrayLR.unlock _at_sep.
+  iIntros "[_ Harr]".
+  rewrite _at_offsetR _at_sub_0; [|done].
+  replace (replicateN n ()) with (replicateN (lengthN xs) ())
+    by (rewrite /replicateN /lengthN -(N2Nat.id n) Hlen; reflexivity).
+  iPoseProof (arrayR_charR_arrayR_anyR with "Harr") as "Harr".
+  rewrite /arrayLR.
+  iSplit.
+  - iPureIntro.
+    unfold lengthZ, lengthN, replicateN.
+    rewrite length_replicate.
+    replace (length xs) with (N.to_nat n) by exact Hlen.
+    repeat rewrite N2Nat.id.
+    lia.
+  - rewrite _at_offsetR _at_sub_0; [|done].
+    iExact "Harr".
+Qed.
+
+Lemma arrayLR_prefix_tail0 `{Σ : cpp_logic, σ : genv}
+    {A : Type} (p : ptr) ty mid hi (R : A -> Rep) xs0 xs1 :
+  lengthN xs0 = Z.to_N mid ->
+  (0 <= mid)%Z ->
+  (mid <= hi)%Z ->
+  p |-> arrayLR ty 0 hi R (xs0 ++ xs1) ⊣⊢
+  p |-> arrayLR ty 0 mid R xs0 ∗
+  p .[ty ! mid] |-> arrayLR ty 0 (hi - mid) R xs1.
+Proof.
+  intros Hlen Hlo Hhi.
+  assert (Hlen' : lengthN xs0 = Z.to_N (mid - 0)) by
+    (replace (mid - 0)%Z with mid by lia; exact Hlen).
+  rewrite (arrayLR_app' p 0 mid hi R xs0 xs1 Hlen' Hlo Hhi).
+  rewrite _at_sub_arrayLR.
+  Arith.arith_simpl.
+  reflexivity.
+Qed.
+
+Lemma arrayR_ucharR_object_bytesR `{Σ : cpp_logic, σ : genv}
+    (p : ptr) xs :
+  p |-> arrayR Tuchar (fun b : Z => ucharR 1$m b) xs ⊢
+  p |-> object_bytesR Tuchar 1$m xs.
+Proof.
+  iIntros "Hs".
+  iApply object_bytesR_of_arrayLR; [reflexivity|].
+  rewrite arrayLR.unlock _at_sep.
+  iSplit; [iPureIntro; lia|].
+  rewrite _at_offsetR _at_sub_0; [iExact "Hs"|done].
+Qed.
+
+Lemma object_bytesR_half_split `{Σ : cpp_logic, σ : genv}
+    (p : ptr) ty bytes :
+  p |-> object_bytesR ty 1$m bytes ⊣⊢
+  p |-> object_bytesR ty (cQp.mk false (1/2)) bytes ∗
+  p |-> object_bytesR ty (cQp.mk false (1/2)) bytes.
+Proof.
+  rewrite -(cfractional (P := fun q => p |-> object_bytesR ty q bytes)
+    (cQp.mk false (1/2)) (cQp.mk false (1/2))).
+  rewrite -cQp.mk_add' Qp.half_half.
+  reflexivity.
+Qed.
+
+Lemma object_bytesR_prefix_tail0 `{Σ : cpp_logic, σ : genv}
+    (p : ptr) ty q mid hi xs0 xs1 :
+  lengthZ (xs0 ++ xs1) = hi ->
+  lengthZ xs0 = mid ->
+  lengthZ xs1 = (hi - mid)%Z ->
+  p |-> object_bytesR ty q (xs0 ++ xs1) ⊣⊢
+  p |-> object_bytesR ty q xs0 ∗
+  p .[ty ! mid] |-> object_bytesR ty q xs1.
+Proof.
+  intros Htotal Hhead Htail.
+  iSplit.
+  - iIntros "Hs".
+    iPoseProof (object_bytesR_to_arrayLR p ty q hi (xs0 ++ xs1)
+      Htotal with "Hs") as "Hs".
+    iPoseProof (arrayLR_prefix_tail0 p ty mid hi
+      (fun b : Z => ucharR q b) xs0 xs1
+      ltac:(rewrite <- Hhead; rewrite N2Z.id; reflexivity)
+      ltac:(lia) ltac:(lia) with "Hs") as "[Hhead Htail]".
+    iPoseProof (object_bytesR_of_arrayLR p ty q mid xs0
+      Hhead with "Hhead") as "Hhead".
+    iPoseProof (object_bytesR_of_arrayLR (p .[ ty ! mid]) ty q
+      (hi - mid) xs1 Htail with "Htail") as "Htail".
+    iFrame.
+  - iIntros "[Hhead Htail]".
+    iPoseProof (object_bytesR_to_arrayLR p ty q mid xs0
+      Hhead with "Hhead") as "Hhead".
+    iPoseProof (object_bytesR_to_arrayLR (p .[ ty ! mid]) ty q
+      (hi - mid) xs1 Htail with "Htail") as "Htail".
+    iPoseProof ((arrayLR_prefix_tail0 p ty mid hi
+      (fun b : Z => ucharR q b) xs0 xs1
+      ltac:(rewrite <- Hhead; rewrite N2Z.id; reflexivity)
+      ltac:(lia) ltac:(lia)) with "[$Hhead $Htail]") as "Hs".
+    iPoseProof (object_bytesR_of_arrayLR p ty q hi
+      (xs0 ++ xs1) Htotal with "Hs") as "Hs".
+    iExact "Hs".
+Qed.
+
+Lemma arrayLR_ucharR_anyR `{Σ : cpp_logic, σ : genv} (p : ptr) n xs :
+  N.to_nat n = length xs ->
+  p |-> arrayLR Tuchar 0 (Z.of_N n) (fun c : Z => ucharR 1$m c) xs ⊢
+  p |-> anyR (Tarray Tuchar n) 1$m.
+Proof.
+  intros Hlen.
+  rewrite arrayLR.unlock _at_sep.
+  iIntros "[_ Harr]".
+  rewrite _at_offsetR _at_sub_0; [|done].
+  rewrite anyR_array.
+  iApply (arrayR_anyR_f (fun c : Z => c) with "Harr").
+  exact Hlen.
+Qed.
+
+Lemma lengthZ_of_to_nat_length {A : Type} (n : N) (xs : list A) :
+  N.to_nat n = length xs -> lengthZ xs = Z.of_N n.
+Proof.
+  intros Hlen.
+  unfold lengthZ, lengthN.
+  rewrite <- Hlen, N2Nat.id.
+  reflexivity.
+Qed.
+
+Lemma memchr_found_after_prefix prefix b suffix c :
+  List.Forall (fun x => x <> byte_of_int c) prefix ->
+  b = byte_of_int c ->
+  memchr (prefix ++ b :: suffix) c = Some (Z.of_nat (length prefix)).
+Proof.
+  intros Hprefix Hb.
+  induction Hprefix as [|x prefix Hx _ IH].
+  - simpl.
+    rewrite bool_decide_true; [|done].
+    reflexivity.
+  - simpl.
+    rewrite bool_decide_false; [|done].
+    rewrite IH.
+    simpl.
+    f_equal.
+    rewrite Nat2Z.inj_succ.
+    rewrite Z.add_1_l.
+    reflexivity.
+Qed.
+
+Lemma memchr_missing_if_no_match bytes c :
+  List.Forall (fun x => x <> byte_of_int c) bytes ->
+  memchr bytes c = None.
+Proof.
+  intros Hbytes.
+  induction Hbytes as [|x bytes Hx _ IH].
+  - reflexivity.
+  - simpl.
+    rewrite bool_decide_false; [|done].
+    rewrite IH.
+    reflexivity.
+Qed.
+
+Ltac solve_memchr_side :=
+  unfold byte_of_int;
+  repeat (rewrite Z.mod_small; [|lia]);
+  match goal with
+  | |- List.Forall _ [] => constructor
+  | |- List.Forall _ (_ :: _) =>
+      constructor; [solve_memchr_side | solve_memchr_side]
+  | |- _ => lia
+  end.
+
+Lemma object_bytesR_ucharR_anyR `{Σ : cpp_logic, σ : genv}
+    (p : ptr) n xs :
+  N.to_nat n = length xs ->
+  p |-> object_bytesR Tuchar 1$m xs ⊢
+  p |-> anyR (Tarray Tuchar n) 1$m.
+Proof.
+  intros Hlen.
+  iIntros "Hs".
+  iPoseProof (object_bytesR_to_arrayLR p Tuchar 1$m (Z.of_N n) xs
+    ltac:(apply lengthZ_of_to_nat_length; exact Hlen)
+    with "Hs") as "Hs".
+  iApply (arrayLR_ucharR_anyR with "Hs").
+  exact Hlen.
+Qed.
+
+Lemma object_bytesR_ucharR_object_bytes_anyR
+    `{Σ : cpp_logic, σ : genv} (p : ptr) n xs :
+  N.to_nat n = length xs ->
+  p |-> object_bytesR Tuchar 1$m xs ⊢
+  p |-> object_bytes_anyR Tuchar (Z.of_N n).
+Proof.
+  intros Hlen.
+  iIntros "Hs".
+  iPoseProof (object_bytesR_ucharR_anyR _ n xs Hlen with "Hs") as "Hs".
+  iApply (object_bytes_anyR_of_anyR_array with "Hs").
+Qed.
+
+Lemma object_bytesR_ucharR_arrayR `{Σ : cpp_logic, σ : genv}
+    (p : ptr) xs :
+  p |-> object_bytesR Tuchar 1$m xs ⊢
+  p |-> arrayR Tuchar (fun b : Z => ucharR 1$m b) xs.
+Proof.
+  iIntros "Hs".
+  iPoseProof (object_bytesR_to_arrayLR p Tuchar 1$m (lengthZ xs) xs
+    eq_refl with "Hs") as "Hs".
+  rewrite arrayLR.unlock _at_sep.
+  iDestruct "Hs" as "[_ Hs]".
+  rewrite _at_offsetR _at_sub_0; [iExact "Hs"|done].
+Qed.
+
+Lemma at_arrayR_ucharR_cons `{Σ : cpp_logic, σ : genv}
+    (p : ptr) x xs :
+  p |-> arrayR Tuchar (fun b : Z => ucharR 1$m b) (x :: xs) ⊣⊢
+  p |-> type_ptrR Tuchar ∗
+  p |-> ucharR 1$m x ∗
+  p .[Tuchar ! 1] |-> arrayR Tuchar (fun b : Z => ucharR 1$m b) xs.
+Proof.
+  rewrite arrayR_cons !_at_sep.
+  rewrite _at_offsetR.
+  reflexivity.
+Qed.
+
+Lemma at_arrayR_cons `{Σ : cpp_logic, σ : genv}
+    {A : Type} (p : ptr) ty (R : A -> Rep) x xs :
+  p |-> arrayR ty R (x :: xs) ⊣⊢
+  p |-> type_ptrR ty ∗
+  p |-> R x ∗
+  p .[ty ! 1] |-> arrayR ty R xs.
+Proof.
+  rewrite arrayR_cons !_at_sep.
+  rewrite _at_offsetR.
+  reflexivity.
+Qed.
+
+Lemma at_ucharR_anyR `{Σ : cpp_logic, σ : genv}
+    (p : ptr) q x :
+  p |-> ucharR q x ⊢ p |-> anyR Tuchar q.
+Proof.
+  apply heap_pred._at_cancel.
+  apply primR_anyR.
+Qed.
+
+Lemma arrayR_ucharR_arrayR_anyR `{Σ : cpp_logic, σ : genv}
+    (p : ptr) xs :
+  p |-> arrayR Tuchar (fun b : Z => ucharR 1$m b) xs ⊢
+  p |-> arrayR Tuchar (fun _ : unit => anyR Tuchar 1$m)
+    (replicateN (lengthN xs) ()).
+Proof.
+  revert p.
+  induction xs as [|x xs IH].
+  all: intros p.
+  - rewrite /lengthN /= !arrayR_nil. reflexivity.
+  - rewrite (at_arrayR_ucharR_cons p x xs).
+    iIntros "(Hty & Hx & Hxs)".
+    replace (lengthN (x :: xs)) with (N.succ (lengthN xs)) by
+      (rewrite /lengthN Nat2N.inj_succ; reflexivity).
+    rewrite replicateN_S.
+    rewrite (at_arrayR_cons p Tuchar
+      (fun _ : unit => anyR Tuchar 1$m) () (replicateN (lengthN xs) ())).
+    iFrame "Hty".
+    iSplitL "Hx".
+    + iApply (at_ucharR_anyR with "Hx").
+    + iApply (IH with "Hxs").
+Qed.
+
+Lemma object_bytesR_ucharR_arrayLR_anyR
+    `{Σ : cpp_logic, σ : genv} (p : ptr) n xs :
+  N.to_nat n = length xs ->
+  p |-> object_bytesR Tuchar 1$m xs ⊢
+  p |-> arrayLR Tuchar 0 (Z.of_N n)
+    (fun _ : unit => anyR Tuchar 1$m) (replicateN n ()).
+Proof.
+  intros Hlen.
+  iIntros "Hs".
+  iPoseProof (object_bytesR_ucharR_arrayR with "Hs") as "Hs".
+  rewrite arrayLR.unlock _at_sep.
+  iSplit.
+  - iPureIntro.
+    unfold lengthZ, lengthN, replicateN.
+    rewrite length_replicate N2Nat.id.
+    lia.
+  - rewrite _at_offsetR _at_sub_0; [|done].
+    rewrite -(N2Nat.id n) Hlen.
+    iApply (arrayR_ucharR_arrayR_anyR with "Hs").
+Qed.
+
+Lemma object_bytesR_arrayLR_cons `{Σ : cpp_logic, σ : genv}
+    (p : ptr) x xs :
+  p |-> object_bytesR Tuchar 1$m (x :: xs) ⊣⊢
+  (type_ptr Tuchar (p .[Tuchar ! 0]) ∗ p .[Tuchar ! 0] |-> ucharR 1$m x) ∗
+  p |-> arrayLR Tuchar 1 (lengthZ (x :: xs)) (fun b : Z => ucharR 1$m b) xs.
+Proof.
+  iSplit.
+  - iIntros "Hs".
+    iPoseProof (object_bytesR_to_arrayLR p Tuchar 1$m (lengthZ (x :: xs))
+      (x :: xs) eq_refl with "Hs") as "Hs".
+    iEval (rewrite (arrayLR_cons p 0 (lengthZ (x :: xs))
+      (fun b : Z => ucharR 1$m b) x xs)) in "Hs".
+    iExact "Hs".
+  - iIntros "[[#Hty Hx] Hs]".
+    iApply (object_bytesR_of_arrayLR p Tuchar 1$m (lengthZ (x :: xs))
+      (x :: xs) eq_refl).
+    rewrite (arrayLR_cons p 0 (lengthZ (x :: xs))
+      (fun b : Z => ucharR 1$m b) x xs).
+    iFrame "# ∗".
+Qed.
+
+Lemma uchar_cells_object_bytesR_two `{Σ : cpp_logic, σ : genv}
+    (p : ptr) a b :
+  p |-> ucharR 1$m a ∗
+  p .[Tuchar ! 1] |-> ucharR 1$m b ⊢
+  p |-> object_bytesR Tuchar 1$m [a; b].
+Proof.
+  iIntros "(Ha & Hb)".
+  iDestruct (observe (p |-> type_ptrR Tuchar) with "Ha") as "#Hty0".
+  iDestruct (observe (p .[Tuchar ! 1] |-> type_ptrR Tuchar) with "Hb")
+    as "#Hty1".
+  iApply arrayR_ucharR_object_bytesR.
+  rewrite (at_arrayR_ucharR_cons p a [b]).
+  iFrame "Hty0 Ha".
+  rewrite (at_arrayR_ucharR_cons (p .[Tuchar ! 1]) b []).
+  iFrame "Hty1 Hb".
+  rewrite arrayR_nil _at_sep.
+  iSplit.
+  - iApply (at_type_ptrR_validR_plus_one with "Hty1").
+  - iPureIntro. done.
+Qed.
+
+Lemma arrayR_ucharR_anyR `{Σ : cpp_logic, σ : genv} (p : ptr) n xs :
+  N.to_nat n = length xs ->
+  p |-> arrayR Tuchar (fun b : Z => ucharR 1$m b) xs ⊢
+  p |-> anyR (Tarray Tuchar n) 1$m.
+Proof.
+  intros Hlen.
+  iIntros "Hs".
+  iPoseProof (arrayR_ucharR_object_bytesR with "Hs") as "Hs".
+  iApply (object_bytesR_ucharR_anyR with "Hs").
+  exact Hlen.
+Qed.
