rocq-brick-libstdcpp/test/cstring/proofs_embedded_null.v
@@ -1,0 +1,158 @@
+(*
+ * Copyright (c) 2026 SkyLabs AI, Inc.
+ * This software is distributed under the terms of the BedRock Open-Source License.
+ * See the LICENSE-BedRock file in the repository root for details.
+ *)
+Require Import skylabs.auto.cpp.proof.
+Require Import skylabs.auto.cpp.hints.anyR.
+(** BEGIN: SKYLABS DEFAULT PROOF IMPORTS *)
+Require Import skylabs.auto.cpp.prelude.proof.
+Require Import skylabs.cpp.array.
+Import expr_join.
+#[local] Hint Resolve delayed_case.smash_delayed_case_B | 1000 : br_hints.
+#[local] Hint Resolve delayed_case.expr_join.smash_delayed_case_B | 1000 : br_hints.
+
+(** END: SKYLABS DEFAULT PROOF IMPORTS *)
+Require Import skylabs.brick.libstdcpp.cassert.spec.
+Require Import skylabs.brick.libstdcpp.cstring.spec.
+Require Import skylabs.brick.libstdcpp.test.cstring.test_cpp.
+
+Import normalize.only_provable_norm.
+
+Import normalize.normalize_ptr.
+Import refine_lib.
+
+Section with_cpp.
+  Context `{Σ : cpp_logic} `{MOD : module ⊧ σ}.
+
+  cpp.spec "test_strlen_embedded_null()" default.
+  Lemma test_strlen_embedded_null_ok :
+    verify[module] "test_strlen_embedded_null()".
+  Admitted.
+
+  cpp.spec "test_strcmp_embedded_null()" default.
+  Lemma test_strcmp_embedded_null_ok :
+    verify[module] "test_strcmp_embedded_null()".
+  Admitted.
+
+  cpp.spec "test_strncmp_embedded_null()" default.
+  Lemma test_strncmp_embedded_null_ok :
+    verify[module] "test_strncmp_embedded_null()".
+  Admitted.
+
+  cpp.spec "test_memset_embedded_null()" default.
+  Lemma test_memset_embedded_null_ok :
+    verify[module] "test_memset_embedded_null()".
+  Proof using MOD _Σ thread_info Σ σ.
+    verify_spec; go.
+    iDestruct select (s_addr |-> arrayLR "unsigned char" (1 + 1) 4
+      (fun v : Z => ucharR 1$m v) [99%Z; 100%Z]) as "Htail".
+    iDestruct select (s_addr .["unsigned char" ! 1] |-> ucharR 1$m 98%Z)
+      as "H1".
+    iDestruct select (s_addr .["unsigned char" ! 0] |-> ucharR 1$m 97%Z)
+      as "H0".
+    iEval (rewrite (arrayLR_cons s_addr 2 4 (fun b : Z => ucharR 1$m b)
+      99%Z [100%Z])) in "Htail".
+    iDestruct "Htail" as "[[#Hty2 H2] Htail]".
+    iPoseProof (at_uchar_offset_add_intro s_addr 1 1 2
+      (ucharR 1$m 99%Z) ltac:(lia) with "H2") as "H2".
+    iPoseProof (uchar_cells_object_bytesR_two (s_addr .[Tuchar ! 1])
+      98%Z 99%Z with "[$H1 $H2]") as "Htarget".
+    iEval (rewrite (arrayLR_cons s_addr 3 4 (fun b : Z => ucharR 1$m b)
+      100%Z [])) in "Htail".
+    iDestruct "Htail" as "[[#Hty3 H3] Hempty]".
+    iExists Tuchar.
+    iSplitL "Htarget".
+    - iApply (object_bytesR_ucharR_object_bytes_anyR _ 2%N
+        [98%Z; 99%Z] ltac:(reflexivity) with "Htarget").
+    - iIntros "Htarget".
+      go.
+      iPoseProof (object_bytesR_arrayLR_cons (s_addr .[Tuchar ! 1]) 0%Z
+        [0%Z] with "Htarget") as "[[#Hty1 H1] Htarget]".
+      iEval (rewrite (arrayLR_cons (s_addr .[Tuchar ! 1]) 1 2
+        (fun b : Z => ucharR 1$m b) 0%Z [])) in "Htarget".
+      iDestruct "Htarget" as "[[#Hty2' H2] Hempty2]".
+      iFrame "H0". iIntros "H0".
+      go.
+      iPoseProof (at_zero_elim (s_addr .[Tuchar ! 1]) with "H1") as "H1".
+      iFrame "H1". iIntros "H1".
+      go.
+      iPoseProof (at_uchar_offset_add_elim s_addr 1 1 2
+        (ucharR 1$m 0%Z) ltac:(lia) with "H2") as "H2".
+      iFrame "H2". iIntros "H2".
+      go.
+      iFrame "H3". iIntros "H3".
+      go.
+      iPoseProof (at_zero_elim s_addr with "H0") as "H0".
+      iPoseProof (uchar_cells_object_bytesR_two s_addr 97%Z 0%Z
+        with "[$H0 $H1]") as "Hhead".
+      iPoseProof (at_uchar_offset_add_intro s_addr 2 1 3
+        (ucharR 1$m 100%Z) ltac:(lia) with "H3") as "H3".
+      iPoseProof (uchar_cells_object_bytesR_two (s_addr .[Tuchar ! 2])
+        0%Z 100%Z with "[$H2 $H3]") as "Htail".
+      iPoseProof ((object_bytesR_prefix_tail0 s_addr Tuchar
+        (cQp.mk false 1) 2 4 [97%Z; 0%Z] [0%Z; 100%Z]
+        ltac:(reflexivity) ltac:(reflexivity) ltac:(reflexivity))
+        with "[$Hhead $Htail]") as "Hs".
+      iPoseProof (object_bytesR_ucharR_arrayLR_anyR _ 4%N
+        [97%Z; 0%Z; 0%Z; 100%Z] ltac:(reflexivity) with "Hs") as "Hs".
+      iFrame "Hs".
+      go.
+  Qed.
+
+  cpp.spec "test_memchr_embedded_null()" default.
+  Lemma test_memchr_embedded_null_ok :
+    verify[module] "test_memchr_embedded_null()".
+  Proof using MOD _Σ thread_info Σ σ.
+    verify_spec; go.
+    iDestruct select (s_addr |-> arrayLR Tuchar 0 4
+      (fun v : Z => ucharR 1$m v) [97%Z; 0%Z; 98%Z; 0%Z]) as "Hs".
+    iPoseProof (object_bytesR_of_arrayLR s_addr Tuchar (cQp.mk false 1)
+      4 [97%Z; 0%Z; 98%Z; 0%Z] ltac:(reflexivity) with "Hs") as "Hs".
+    iExists Tuchar, (cQp.mk false 1), [97%Z; 0%Z; 98%Z; 0%Z].
+    iSplitL "Hs"; [iExact "Hs"|].
+    iSplit.
+    + done.
+    + iIntros "Hs".
+      rewrite (memchr_found_after_prefix [97%Z] 0%Z [98%Z; 0%Z] 0%Z); [|solve_memchr_side..].
+      Arith.arith_simpl; go.
+    iPoseProof (object_bytesR_prefix_tail0 s_addr Tuchar
+      (cQp.mk false 1) 2 4 [97%Z; 0%Z] [98%Z; 0%Z]
+      ltac:(reflexivity) ltac:(reflexivity) ltac:(reflexivity) with "Hs")
+      as "[Hhead Hs]".
+    iExists Tuchar, (cQp.mk false 1), [98%Z; 0%Z].
+    iSplitL "Hs"; [iExact "Hs"|].
+    iSplit; [done|].
+    iIntros "Hs".
+    rewrite (memchr_found_after_prefix [98%Z] 0%Z (@nil Z) 0%Z); [|solve_memchr_side..].
+    Arith.arith_simpl; go.
+    rewrite o_sub_sub.
+    Arith.arith_simpl.
+    go.
+    iPoseProof ((object_bytesR_prefix_tail0 s_addr Tuchar
+      (cQp.mk false 1) 2 4 [97%Z; 0%Z] [98%Z; 0%Z]
+      ltac:(reflexivity) ltac:(reflexivity) ltac:(reflexivity))
+      with "[$Hhead $Hs]")
+      as "Hs".
+    iExists Tuchar, (cQp.mk false 1), [97%Z; 0%Z; 98%Z; 0%Z].
+    iSplitL "Hs"; [iExact "Hs"|].
+    iSplit; [done|].
+    iIntros "Hs".
+    rewrite (memchr_found_after_prefix [97%Z; 0%Z] 98%Z [0%Z] 98%Z); [|solve_memchr_side..].
+    Arith.arith_simpl; go.
+    iPoseProof (object_bytesR_ucharR_arrayLR_anyR _ 4%N
+      [97%Z; 0%Z; 98%Z; 0%Z]
+      ltac:(reflexivity) with "Hs") as "Hs".
+    iFrame "Hs".
+    go.
+    rewrite o_sub_sub in H.
+    simpl in H.
+    contradiction.
+  Qed.
+
+  cpp.spec "test_memcmp_embedded_null()" default.
+
+  cpp.spec "test_memcpy_embedded_null()" default.
+
+  cpp.spec "test_memmove_embedded_null()" default.
+End with_cpp.
